src/Examples/DnsServer/DnsLemmas.v
@@ -820,3 +820,75 @@ this is because x is a list of tuples that all came from r *)
   apply Equiv' in H15; destruct H15;  apply H15.
   apply DecideableEnsemble_bool.
 Qed.
+
+Lemma refine_beq_RRecordType_dec :
+  forall rr : resourceRecord,
+    refine {b | decides b (rr!sTYPE = CNAME)}
+           (ret (beq_RRecordType rr!sTYPE CNAME)).
+Proof.
+  intros; rewrite <- beq_RRecordType_dec.
+  intros; refine pick val _.
+  finish honing.
+  find_if_inside; simpl; eauto.
+Qed.
+
+Lemma refine_noDup_CNAME_check :
+  forall (rr : resourceRecord)
+         (R : @IndexedEnsemble resourceRecord),
+  (forall tup tup' : IndexedElement,
+          elementIndex tup <> elementIndex tup' ->
+          R tup ->
+          R tup' ->
+          (indexedElement tup)!sNAME = (indexedElement tup')!sNAME
+          -> (indexedElement tup)!sTYPE <> CNAME)
+  -> refine {b |
+            decides b
+                    (forall tup',
+                        R tup' ->
+                        rr!sNAME = (indexedElement tup')!sNAME -> rr!sTYPE <> CNAME)}
+           (If (beq_RRecordType rr!sTYPE CNAME)
+               Then count <- Count
+               For
+               (QueryResultComp R
+                                (fun tup => Where (rr!sNAME = tup!sNAME)
+                                                  Return tup )%QueryImpl);
+                  ret (beq_nat count 0) Else ret true).
+Proof.
+  intros.
+    intros; setoid_rewrite refine_pick_decides at 1;
+    [ | apply refine_is_CNAME__forall_to_exists | apply refine_not_CNAME__independent ].
+    setoid_rewrite refine_beq_RRecordType_dec; simplify with monad laws.
+    apply refine_If_Then_Else; eauto.
+    setoid_rewrite refine_constraint_check_into_QueryResultComp with (P := fun tup => rr!sNAME = tup!sNAME).
+    rewrite refineEquiv_bind_bind.
+    f_equiv.
+    unfold pointwise_relation; intros; simplify with monad laws;
+      rewrite <- negb_involutive_reverse; reflexivity.
+    auto with typeclass_instances.
+    intuition.
+    reflexivity.
+Qed.
+
+Corollary refine_noDup_CNAME_check_dns :
+  forall (rr : resourceRecord) r_o r_n,
+    @DropQSConstraints_AbsR DnsSchema r_o r_n
+  -> refine {b |
+            decides b
+                    (forall tup',
+                        (GetUnConstrRelation r_n Fin.F1) tup' ->
+                        rr!sNAME = (indexedElement tup')!sNAME -> rr!sTYPE <> CNAME)}
+           (If (beq_RRecordType rr!sTYPE CNAME)
+               Then count <- Count
+               For
+               (UnConstrQuery_In r_n Fin.F1
+                                (fun tup => Where (rr!sNAME = tup!sNAME)
+                                                  Return tup )%QueryImpl);
+                  ret (beq_nat count 0) Else ret true).
+Proof.
+  intros; eapply refine_noDup_CNAME_check.
+  intros; eapply (DropQSConstraints_AbsR_SatisfiesTupleConstraints H Fin.F1); eauto.
+Qed.
+
+Instance ADomainName_eq : Query_eq DomainName := Astring_eq.
+Instance ARRecordType_eq : Query_eq RRecordType :=
+  {| A_eq_dec := fin_eq_dec |}.
