src/Examples/DnsServer/Packet.v
@@ -42,18 +42,8 @@ Section QTypes.
     ].
 
   Definition QType_Ws : t (word 16) 17 :=
-    Eval simpl in Vector.map (natToWord 16)
-                             [1; (* "A" *)
-                                2; (* "NS" *)
-                                5; (* "CNAME" *)
-                                6; (* "SOA"*)
-                                11; (* "WKS" *)
-                                12; (* "PTR" *)
-                                13; (* "HINFO" *)
-                                14; (* "MINFO" *)
-                                15; (* "MX" *)
-                                16; (* "TXT" *)
-                                249; (*"TKEY" *)
+    Eval simpl in RRecordType_Ws ++ Vector.map (natToWord 16)
+                             [249; (*"TKEY" *)
                                 250; (*"TSIG" *)
                                 251; (*"IXFR" *)
                                 252; (*"AXFR" *)
@@ -98,7 +88,7 @@ Section RRecordClass.
                              [1; (* "IN" *)
                                 3; (* "CH" *)
                                 4 (* "Hesiod" *)].
-  
+
   Definition RRecordClass := EnumType RRecordClasses.
 
   Definition beq_RRecordClass (a b : RRecordClass) : bool
@@ -113,8 +103,8 @@ Section RRecordClass.
   Definition QClass_Ws : t (word 16) 4 :=
     Eval simpl in Vector.append
                     RRecordClass_Ws
-                    [natToWord 16 255 (* "Any"*)].  
-  
+                    [natToWord 16 255 (* "Any"*)].
+
   Definition QClass_inj (qclass : RRecordClass) : QClass :=
     Fin.L _ qclass.
 
@@ -139,11 +129,11 @@ Section ResponseCode.
        "YXRRSet";  (* RR Set Exists when it should not 	[RFC2136] *)
        "NXRRSet";  (* RR Set that should exist does not 	[RFC2136] *)
        "NotAuth";  (* Server Not Authoritative for zone 	[RFC2136] *)
-       "NotAuth";  (* Not Authorized [RFC2845] *)
+                   (* and Not Authorized [RFC2845] *)
        "NotZone" 	 (* Name not  contained in zone 	[RFC2136] *)
     ].
 
-  Definition RCODE_Ws : t (word 4) 12 :=
+  Definition RCODE_Ws : t (word 4) 11 :=
     Eval simpl in Vector.map (natToWord 4)
     [0;  (* No Error [RFC1035] *)
      1;  (* Format Error [RFC1035] *)
@@ -155,10 +145,10 @@ Section ResponseCode.
      7;  (* RR Set Exists when it should not 	[RFC2136] *)
      8;  (* RR Set that should exist does not 	[RFC2136] *)
      9;  (* Server Not Authoritative for zone 	[RFC2136] *)
-     9;  (* Not Authorized [RFC2845] *)
+         (* and Not Authorized [RFC2845] *)
      10 	 (* Name not  contained in zone 	[RFC2136] *)
     ].
-  
+
   Definition ResponseCode := EnumType ResponseCodes.
 
   Definition beq_ResponseCode (a b : ResponseCode) : bool
@@ -185,7 +175,7 @@ Section OpCode.
                               1; (* Inverse Query  OBSOLETE) [RFC3425] *)
                               2; (* [RFC1035] *)
                               4  (* [RFC1996] [RFC2136] *)].
- 
+
   Definition beq_OpCode (a b : OpCode) : bool
     := fin_beq a b.
 
@@ -331,14 +321,14 @@ Definition ID : Type := word 16.
   Definition packet := @Tuple packetHeading.
 
   Definition buildempty (is_authority : bool)
-             (rcode : ResponseCode)
+             (rcode : BoundedIndex ResponseCodes)
              (p : packet) :=
     p ○ [ "AA" ::= is_authority; (* Update Authority field *)
-            "QR" ::= true; (* Set response flag to true *)
-            "RCODE" ::= rcode;
-            "answers" ::= nil;
-            "authority"  ::= nil;
-            "additional" ::= nil ].
+          "QR" ::= true; (* Set response flag to true *)
+          "RCODE" ::= ibound (indexb rcode);
+          "answers" ::= nil;
+          "authority"  ::= nil;
+          "additional" ::= nil ].
 
   (* add a resource record to a packet's answers *)
   Definition add_answer (p : packet) (t : resourceRecord) :=
